WIP

coq-minuska/theories/builtin/information_flow_functor.v
@@ -7,7 +7,52 @@ From Minuska Require Import
 
 From stdpp Require Import decidable.
 
-Class IFCRelaxedModelTrait
+Class IFLattice (TagType : Type) := {
+    ifl_meet :
+        TagType -> TagType -> TagType
+    ;
+    ifl_meet_assoc ::
+        Assoc (=) ifl_meet
+    ;
+    ifl_meet_comm ::
+        Comm (=) ifl_meet
+    ;
+
+    ifl_join :
+        TagType -> TagType -> TagType
+    ;
+    ifl_join_assoc ::
+        Assoc (=) ifl_join
+    ;
+    ifl_join_comm ::
+        Comm (=) ifl_join
+    ;
+
+    ifl_absorb_1 :
+        forall a b, ifl_join a (ifl_meet a b) = a
+    ;
+
+    ifl_absorb_2 :
+        forall a b, ifl_meet a (ifl_join a b) = a
+    ;
+
+    ifl_bot : TagType ;
+
+    ifl_join_bot :
+        forall a,
+        ifl_join ifl_bot a = a
+    ;
+
+    ifl_top : TagType ; 
+
+    ifl_meet_top :
+        forall a,
+        ifl_meet ifl_top a = a
+    ;
+}.
+
+
+Class IFCRelaxedModelTrait0
     (TagType : Type)
     {_E : EqDecision TagType}
     {_C : Countable TagType}
@@ -16,12 +61,23 @@ Class IFCRelaxedModelTrait
     {signature : Signature}
     {NondetValue : Type}
     {FromT : Type}
+    {_EF : EqDecision FromT}
     (Morig : RelaxedModel signature NondetValue FromT)
     (Miflow : RelaxedModel signature NondetValue FromT)
 := {
-    ifc_tagged : @rm_carrier _ _ _ _ _ Morig -> gset TagType -> @rm_carrier _ _ _ _ _ Miflow ;
-    ifc_get_tags : @rm_carrier _ _ _ _ _ Miflow -> gset TagType ;
-    ifc_get_pure : @rm_carrier _ _ _ _ _ Miflow -> @rm_carrier _ _ _ _ _ Morig ;
+    ifc_tagged :
+        @rm_carrier _ _ _ _ _ Morig ->
+        gset TagType ->
+        @rm_carrier _ _ _ _ _ Miflow
+    ;
+    ifc_get_tags :
+        @rm_carrier _ _ _ _ _ Miflow ->
+        gset TagType
+    ;
+    ifc_get_pure :
+        @rm_carrier _ _ _ _ _ Miflow ->
+        @rm_carrier _ _ _ _ _ Morig
+    ;
 
     ifc_get_tags_of_tagged :
         forall c tags,
@@ -162,7 +218,7 @@ Program Instance information_flow_functor_trait
     {NondetValue : Type}
     (M : @RelaxedModel symbol symbols signature NondetValue void)
     :
-    IFCRelaxedModelTrait TagType M (rmf_apply (information_flow_functor TagType) M)
+    IFCRelaxedModelTrait0 TagType M (rmf_apply (information_flow_functor TagType) M)
 := {|
     ifc_tagged := information_flow_functor_tagged TagType M ;
     ifc_get_tags := information_flow_functor_get_tags TagType M;
@@ -180,4 +236,163 @@ Next Obligation.
 Qed.
 Fail Next Obligation.
 
+Definition eval_predicate_in_orig
+    {TagType : Type}
+    {_E : EqDecision TagType}
+    {_C : Countable TagType}
+    {symbol : Type}
+    {symbols : Symbols symbol}
+    {signature : Signature}
+    {NondetValue : Type}
+    {FromT : Type}
+    {_EF : EqDecision FromT}
+    {Morig : RelaxedModel signature NondetValue FromT}
+    {Miflow : RelaxedModel signature NondetValue FromT}
+    (trait0 : IFCRelaxedModelTrait0 TagType Morig Miflow)
+    (Carrier : Type)
+    (inja : Injection FromT Carrier)
+    (injb : ReversibleInjection (@rm_carrier _ _ _ _ _ Morig) Carrier)
+    (p : builtin_predicate_symbol)
+    (nv : NondetValue)
+    (args : list (TermOver' (@rm_carrier _ _ _ _ _ Miflow)))
+:=
+    let args' : list (TermOver' (@rm_carrier _ _ _ _ _ Morig)) := (list_fmap _ _ (TermOver'_map ifc_get_pure) args) in
+    let args'' : list (TermOver' Carrier) := list_fmap _ _ (TermOver'_map (@inject _ _ (@ri_injection _ _ injb))) args' in
+    @builtin_predicate_interp _ _ _ _ _ (@rm_model_over _ _ signature _ _ Morig Carrier inja injb) p nv args''
+.
+
+Definition eval_predicate_in_iflow
+    {TagType : Type}
+    {_E : EqDecision TagType}
+    {_C : Countable TagType}
+    {symbol : Type}
+    {symbols : Symbols symbol}
+    {signature : Signature}
+    {NondetValue : Type}
+    {FromT : Type}
+    {_EF : EqDecision FromT}
+    {Morig : RelaxedModel signature NondetValue FromT}
+    {Miflow : RelaxedModel signature NondetValue FromT}
+    (trait0 : IFCRelaxedModelTrait0 TagType Morig Miflow)
+    (Carrier : Type)
+    (inja : Injection FromT Carrier)
+    (injb : ReversibleInjection (@rm_carrier _ _ _ _ _ Miflow) Carrier)
+    (p : builtin_predicate_symbol)
+    (nv : NondetValue)
+    (args : list (TermOver' (@rm_carrier _ _ _ _ _ Miflow)))
+:=
+    let args' := (TermOver'_map (@inject _ _ (@ri_injection _ _ injb))) <$> args in
+    @builtin_predicate_interp _ _ _ _ _ (@rm_model_over _ _ signature _ _ Miflow Carrier inja injb) p nv args'
+.
+
+
+Definition eval_function_in_orig
+    {TagType : Type}
+    {_E : EqDecision TagType}
+    {_C : Countable TagType}
+    {symbol : Type}
+    {symbols : Symbols symbol}
+    {signature : Signature}
+    {NondetValue : Type}
+    {FromT : Type}
+    {_EF : EqDecision FromT}
+    {Morig : RelaxedModel signature NondetValue FromT}
+    {Miflow : RelaxedModel signature NondetValue FromT}
+    (trait0 : IFCRelaxedModelTrait0 TagType Morig Miflow)
+    (Carrier : Type)
+    (inja : Injection FromT Carrier)
+    (injb : ReversibleInjection (@rm_carrier _ _ _ _ _ Morig) Carrier)
+    (f : builtin_function_symbol)
+    (nv : NondetValue)
+    (args : list (TermOver' (@rm_carrier _ _ _ _ _ Miflow)))
+    :
+    TermOver' Carrier
+:=
+    let args' : list (TermOver' (@rm_carrier _ _ _ _ _ Morig)) := (list_fmap _ _ (TermOver'_map ifc_get_pure) args) in
+    let args'' : list (TermOver' Carrier) := list_fmap _ _ (TermOver'_map (@inject _ _ (@ri_injection _ _ injb))) args' in
+    @builtin_function_interp _ _ _ _ _ (@rm_model_over _ _ signature _ _ Morig Carrier inja injb) f nv args''
+.
+
+Definition eval_function_in_iflow
+    {TagType : Type}
+    {_E : EqDecision TagType}
+    {_C : Countable TagType}
+    {symbol : Type}
+    {symbols : Symbols symbol}
+    {signature : Signature}
+    {NondetValue : Type}
+    {FromT : Type}
+    {_EF : EqDecision FromT}
+    {Morig : RelaxedModel signature NondetValue FromT}
+    {Miflow : RelaxedModel signature NondetValue FromT}
+    (trait0 : IFCRelaxedModelTrait0 TagType Morig Miflow)
+    (Carrier : Type)
+    (inja : Injection FromT Carrier)
+    (injb : ReversibleInjection (@rm_carrier _ _ _ _ _ Miflow) Carrier)
+    (f : builtin_function_symbol)
+    (nv : NondetValue)
+    (args : list (TermOver' (@rm_carrier _ _ _ _ _ Miflow)))
+    :
+    TermOver' Carrier
+:=
+    let args' := (TermOver'_map (@inject _ _ (@ri_injection _ _ injb))) <$> args in
+    @builtin_function_interp _ _ _ _ _ (@rm_model_over _ _ signature _ _ Miflow Carrier inja injb) f nv args'
+.
+
+
 (* TODO need "the rest" of the natural transformation *)
+Class IFCRelaxedModelTrait1
+    (TagType : Type)
+    {_SL : IFLattice TagType}
+    {_E : EqDecision TagType}
+    {_C : Countable TagType}
+    {symbol : Type}
+    {symbols : Symbols symbol}
+    {signature : Signature}
+    {NondetValue : Type}
+    {FromT : Type}
+    {_EF : EqDecision FromT}
+    (Morig : RelaxedModel signature NondetValue FromT)
+    (Miflow : RelaxedModel signature NondetValue FromT)
+:= {
+
+    ifc_0 :: IFCRelaxedModelTrait0 TagType Morig Miflow ;
+
+    ifc_pure_predicate:
+        forall
+            (Carrier Carrier' : Type)
+            (inja : Injection FromT Carrier)
+            (inja' : Injection FromT Carrier')
+            (injb : ReversibleInjection (@rm_carrier _ _ _ _ _ Morig) Carrier)
+            (injb' : ReversibleInjection (@rm_carrier _ _ _ _ _ Miflow) Carrier'),
+        forall
+            (p : builtin_predicate_symbol)
+            (nv : NondetValue)
+            args,
+        eval_predicate_in_iflow ifc_0 Carrier' inja' injb' p nv args
+        =
+        eval_predicate_in_orig ifc_0 Carrier inja injb p nv args
+    ;
+
+    ifc_pure_function:
+        forall
+            (Carrier Carrier' : Type)
+            (inja : Injection FromT Carrier)
+            (inja' : Injection FromT Carrier')
+            (injb : ReversibleInjection (@rm_carrier _ _ _ _ _ Morig) Carrier)
+            (injb' : ReversibleInjection (@rm_carrier _ _ _ _ _ Miflow) Carrier'),
+        forall
+            (f : builtin_function_symbol)
+            (nv : NondetValue)
+            args,
+        let r1 := eval_function_in_iflow ifc_0 Carrier' inja' injb' f nv args in
+        let r2 := eval_function_in_orig ifc_0 Carrier inja injb f nv args in
+        (* TODO we need to relate the two somehow *)
+        True
+        (* match @ri_reverse _ _ injb r1, ri_reverse r2 with
+        | Some r'1, Some r'2 => False
+        | _,_ => True
+        end *)
+    ;
+}.
+    
